trial proof for h_last_in_trail

VerifiedCdclDatastructures/Solver.lean
@@ -111,35 +111,33 @@ def bcpTest1 : Solver f1.num_vars f1.clauses.size × BCPResult f1.num_vars f1.cl
 -- Then just by transitivity, you have it!
 
 abbrev PropTriple (nv nc : Nat) := Solver nv nc × Array (Fin nc) × Array (Fin nc)
-def ptContingentCt (pt : PropTriple nv nc) : Nat := pt.1.contingent_ct
-
-def propNonUnit (lit : Lit) (in_prop : PropTriple nv nc) (uci : Fin nc) : PropTriple nv nc :=
-  let (s', units', non_uc') := in_prop
+def propNonUnit (lit : Lit) (in_prop : PropTriple nv nc) (i : Fin nc) : PropTriple nv nc :=
+  let (s', units', non_uc) := in_prop
   -- Maybe we could pass proof values around in the solver :)
   -- These clauses are just my attempt at exploring what would satisfy
   -- Lean's bound-checking requirements.
-  let prop_clause := s'.clauses.clauses[uci]
-  if ¬(s'.is_satisfied[uci])
+  let prop_clause := s'.clauses.clauses[i]
+  if ¬(s'.is_satisfied[i])
   then if prop_clause.lits.contains lit
-    then ({ s' with is_satisfied := s'.is_satisfied.set uci true
+    then ({ s' with is_satisfied := s'.is_satisfied.set i true
                     contingent_ct := s'.contingent_ct - 1
-    }, units', non_uc'.push uci)
+    }, units', non_uc.push i)
     else if prop_clause.lits.contains (-lit)
       then 
-        let s' : Solver nv nc := { s' with clauses := s'.clauses.propLit uci }
-        let (units', non_uc) := if s'.clauses.num_unassigned[uci] = 1 
-          then (units'.push uci, non_uc')
-          else (units', non_uc'.push uci)
+        let s' : Solver nv nc := { s' with clauses := s'.clauses.propLit i }
+        let (units', non_uc) := if s'.clauses.num_unassigned[i] = 1 
+          then (units'.push i, non_uc)
+          else (units', non_uc.push i)
         (s', units', non_uc)
-      else (s', units', non_uc'.push uci)
+      else (s', units', non_uc.push i)
   -- Skip the next non-unit
-  else (s', units', non_uc')
+  else (s', units', non_uc)
 
 -- I feel like this proof could be much terser, but throwing dynamite is a martial art as long as it works :)
 -- We want to show that `contingent_ct` always decreases in each call of `bcp`.
 -- This is the ground floor of the proof: show `propNonUnit` doesn't increase contingent_ct.
-lemma propNonUnit_leq (lit : Lit) (pt : PropTriple nv nc) :
-    ∀ uci, (propNonUnit lit pt uci).fst.contingent_ct ≤ pt.fst.contingent_ct := by
+lemma propNonUnit_leq (pt : PropTriple nv nc) :
+    ∀ lit i, (propNonUnit lit pt i).fst.contingent_ct ≤ pt.fst.contingent_ct := by
   intros
   unfold propNonUnit
   split -- destruct match
@@ -150,6 +148,10 @@ lemma propNonUnit_leq (lit : Lit) (pt : PropTriple nv nc) :
       · split -- destruct if
         all_goals simp -- Just simplify both cases thx
     · simp
+
+lemma propNonUnit_leq_foldl_induction (pt : PropTriple nv nc) :
+    ∀ lit (non_uc : Array (Fin nc)), (non_uc.foldl (propNonUnit lit) pt).fst.contingent_ct ≤ pt.fst.contingent_ct := by
+  sorry
 
 def propOne (in_prop : PropTriple nv nc) (uci : Fin nc) : PropTriple nv nc :=
   let (s, units', non_uc') := in_prop
@@ -182,8 +184,7 @@ lemma propOne_lt (pt : PropTriple nv nc) {hcz : pt.fst.contingent_ct > 0} :
     have hcm : s.contingent_ct = s'.contingent_ct - 1 := rfl
     have hc : s.contingent_ct < s'.contingent_ct := by omega
     let s'' := (Array.foldl (propNonUnit lit) (s, #[], #[]) non_uc').fst
-    have hleq : s''.contingent_ct ≤ s.contingent_ct := Array.foldl_leq_monotone non_uc' (propNonUnit lit) (s, #[], #[]) ptContingentCt (propNonUnit_leq lit)
-    -- This proof state will damage your retinas... and hurt your soul
+    have hleq : s''.contingent_ct ≤ s.contingent_ct := propNonUnit_leq_foldl_induction (s, #[], #[]) lit non_uc'
     subst s'' s
     omega
 
@@ -192,12 +193,13 @@ def propUnits (in_prop : PropTriple nv nc) (hc : in_prop.fst.contingent_ct > 0) 
   let (uc_inds, non_uc) := in_prop.snd
   let (s', uc_inds, non_uc) := uc_inds.foldl propOne (s, #[], #[])
 
+  -- Once again, `foldl` induction. Still wrapping my head around exactly what a "motive" is
   have hcc : s'.contingent_ct < s.contingent_ct := by admit
     -- subst s
     -- apply propOne_lt after_prop hc
 
   -- If we don't discover any more unit clauses, we are done propagating. Now to pass judgment.
-  if huc : uc_inds.isEmpty
+  if uc_inds.isEmpty
     then if hcz : s.contingent_ct = 0
       then .ok s
       else match s.clauses.num_unassigned.findFinIdx? (· == 0) with
@@ -206,7 +208,7 @@ def propUnits (in_prop : PropTriple nv nc) (hc : in_prop.fst.contingent_ct > 0) 
                         else .ok s
         | _ => .ok s
     else 
-      -- This is implied by ¬uc_inds.isEmpty.
+      -- This is implied by uc_inds != empty.
       have hcz : s'.contingent_ct > 0 := sorry
       propUnits (s', uc_inds, non_uc) hcz
   termination_by (in_prop.fst.contingent_ct)
@@ -290,20 +292,18 @@ theorem popVar_trail_size_decreases (s : Solver nv nc) (v : Var) :
 lemma last_assigned_lit_in_trail
   (s : Solver nv nc) (curr : CDCL.Clause)
   (h_curr_assigned : ∀ l ∈ curr.lits, containsVar l.var s.trail.stack = true)
-  (last_assigned_lit : CDCL.Lit)
-  (h_last : last_assigned_lit = -(AssignmentTrail.findLastAssigned s.trail curr).get!) :
-    containsVar last_assigned_lit.var s.trail.stack = true := by
-      rw [h_last]
-      have h_found_in_curr : (AssignmentTrail.findLastAssigned s.trail curr).get! ∈ curr.lits := by
-        apply AssignmentTrail.findLastAssigned_returns_lit_in_clause
-        rfl
-      have h_found_var_in_trail : containsVar ((AssignmentTrail.findLastAssigned s.trail curr).get!).var s.trail.stack = true := by
+  (h_last': AssignmentTrail.findLastAssigned s.trail curr = some optional_last_lit) :
+    containsVar optional_last_lit.var s.trail.stack = true := by
+      have h_found_in_curr : optional_last_lit ∈ curr.lits := by
+        apply AssignmentTrail.findLastAssigned_returns_lit_in_clause s.trail
+        rw [h_last']
+        -- rfl
+      have h_found_var_in_trail : containsVar optional_last_lit.var s.trail.stack = true := by
         apply h_curr_assigned
         exact h_found_in_curr
-      -- negation doesn't change variable
       simp only [Lit.var]
       rw [AssignmentTrail.lit_neg_same_var]
-      simp only [Int.neg_neg]
+      simp
       exact h_found_var_in_trail
 
 /- Stub for clause learning. Use this for 1-UIP, it takes
@@ -343,15 +343,15 @@ def learn {nv nc : Nat} (s : Solver nv nc) (conflict : Clause)
       -- NOTE: Can we guarantee that last_assigned_lit is never 0? That we always find last_assigned_lit?
       -- need to show that for all clauses found by pickIncomingEdge, last assigned variable is in trail
       -- and last assigned in curr\{last_assigned_lit} is also in trail
-      let last_assigned_lit := -(AssignmentTrail.findLastAssigned s.trail curr).get!
+      let last_assigned_lit := (AssignmentTrail.findLastAssigned s.trail curr).get!
       -- pick incoming edge
-      let (clause_that_implied, clause_idx) := pickIncomingEdge s last_assigned_lit seenClauses
+      let (clause_that_implied, clause_idx) := pickIncomingEdge s (-last_assigned_lit) seenClauses
       -- resolve clause_that_implied and curr
       -- NOTE: we know that last_assigned_lit's sign in curr is the opposite of its sign in
       -- clause_that_implied
 
       -- TODO: Figure out if this correctly shadows
-      let curr := resolveOnVar curr clause_that_implied last_assigned_lit.var
+      let curr' := resolveOnVar curr clause_that_implied last_assigned_lit.var
       -- update seen clauses
       let seenClauses := seenClauses.insert clause_idx
 
@@ -359,26 +359,38 @@ def learn {nv nc : Nat} (s : Solver nv nc) (conflict : Clause)
       -- NOTE: Do we know that last_assigned_lit is in s.trail before the pop?
       let s' : Solver nv nc := { s with trail := s.trail.popVar last_assigned_lit.var }
 
-     have h_last_in_trail : containsVar last_assigned_lit.var s.trail.stack = true := by
-       apply last_assigned_lit_in_trail
-       · exact h_curr_assigned
-       · rfl
+
+
+      -- TODO: Use last_assigned_lit_in_trail
+      have h_last_in_trail : containsVar last_assigned_lit.var s.trail.stack = true := by
+        -- apply last_assigned_lit_in_trail
+        -- · exact h_curr_assigned
+        -- · 
+        cases h : s.trail.findLastAssigned curr
+        case none => sorry -- should be impossible (PROVE?)
+        case some val =>
+          have h_val_in_trail : containsVar val.var s.trail.stack = true := by
+            apply last_assigned_lit_in_trail s curr
+            · exact h_curr_assigned
+            · apply h
+        simp only [last_assigned_lit, h, Option.get!_some]
+        exact h_val_in_trail
 
       have : s'.trail.size < s.trail.size := by
         simp only [s']
         apply AssignmentTrail.popVar_size_lt_containsVar
         exact h_last_in_trail
 
-      have h_curr'_assigned : ∀ l ∈ curr.lits, containsVar l.var s'.trail.stack = true := by
+      have h_curr'_assigned : ∀ l ∈ curr'.lits, containsVar l.var s'.trail.stack = true := by
         intro l hl
         -- l came from either curr or clause_that_implied but not last_assigned_lit.var, since
         -- it was resolved over
         -- both had all vars in s.trail (prove?)
-        -- we only removed last_assigned_lit
+        -- we only removed last_assigned_littom
         -- so l.var is still in s.trail (PROVE)
         sorry
 
-      loop s' curr seen h_curr'_assigned -- FIXME: Need to prove this recurses correctly, show termination!
+      loop s' curr' seen h_curr'_assigned -- FIXME: Need to prove this recurses correctly, show termination!
   termination_by s.trail.size
 
   let curr : Clause := { conflict with lits := conflict.lits.map (λ l => -l) }
@@ -405,6 +417,9 @@ def secondMax (xs : Array Nat) : Option Nat :=
       else if x >= m2 then (m1, x)
       else (m1, m2)
   some max2
+
+#eval secondMax #[1, 5, 3, 4, 5]  -- some 5
+#eval secondMax #[7]              -- none
 
 -- want 2nd highest dl
 def computeBackjumpLevel {nv nc : Nat} (s : Solver nv nc) (conflict : Clause) : Nat :=
@@ -494,15 +509,11 @@ def solve? {nv nc : Nat} [heur : Heuristic (nv := nv) (nc := nc) α] (s : Solver
   match bcp s hc with
   | Except.ok s' =>
     -- This assignment satisfies all clauses!
-    if hc' : s'.contingent_ct = 0 then
+    if hc : s'.contingent_ct = 0 then
        Except.ok s'.assignment
     else
       -- branching!
-      -- TODO: Pull this proof out-of-line, this thing is ugly!
-      have hbcp : s'.contingent_ct < s.contingent_ct := by 
-        -- apply neq_zero_gt at hc'
-        -- apply bcp_decreases_ct s hc
-        admit
+      have hbcp : s'.contingent_ct < s.contingent_ct := bcp_decreases_ct s hc
       let s_w_decide := decide (α := α) s'
       have hd : s'.contingent_ct = s_w_decide.contingent_ct := by
         simp_all
@@ -511,8 +522,6 @@ def solve? {nv nc : Nat} [heur : Heuristic (nv := nv) (nc := nc) α] (s : Solver
         apply decide_preserves_ct s'
       have hc : s_w_decide.contingent_ct > 0 := by
         simp_all
-        omega
-      have : s_w_decide.contingent_ct < s.contingent_ct := by
         omega
 
       solve? (α := α) s_w_decide (hc := hc)
@@ -527,7 +536,6 @@ def solve? {nv nc : Nat} [heur : Heuristic (nv := nv) (nc := nc) α] (s : Solver
       let s''' := backjump s'' backjumpLvl
       -- TODO: Backjumping will, by defintion, make 
       have hb : s'''.contingent_ct > 0 := sorry
-      have : s'''.contingent_ct < s.contingent_ct := sorry
       solve? (α := α) s''' (hc := hb)
   termination_by (s.contingent_ct)
 
